feat: preservation_subst

CollapsingTowers/TwoLevelPCP/OpenClose.lean
@@ -105,8 +105,7 @@ def closedb_at (e : Expr) (b : ℕ) : Prop :=
   | .let𝕔 e1 e2 => closedb_at e1 b ∧ closedb_at e2 (b + 1)
 
 @[simp]
-def lc e :=
-  closedb_at e 0
+def lc e := closedb_at e 0
 
 @[simp]
 def maping𝕔 (e : Expr) (i : ℕ) : Expr :=
@@ -127,5 +126,521 @@ def maping𝕔 (e : Expr) (i : ℕ) : Expr :=
   | .let𝕔 b e => .let𝕔 (maping𝕔 b i) (maping𝕔 e (i + 1))
 
 @[simp]
-def map𝕔₀ (e : Expr) : Expr :=
-  maping𝕔 e 0
+def map𝕔₀ (e : Expr) : Expr := maping𝕔 e 0
+
+-- Properties
+lemma subst_intro : ∀ x e v i, closed_at e x → subst x v (opening i (.fvar x) e) = opening i v e :=
+  by
+  intros _ e _ i Hclosed
+  induction e generalizing i with
+  | bvar j =>
+    by_cases HEq : j = i
+    . simp [HEq]
+    . simp [if_neg HEq]
+  | fvar y =>
+    simp at *; omega
+  | lam₁ _ IHe
+  | lift _ IHe
+  | code _ IHe
+  | reflect _ IHe
+  | lam𝕔 _ IHe =>
+    simp; apply IHe; apply Hclosed
+  | app₁ _ _ IH₀ IH₁
+  | app₂ _ _ IH₀ IH₁
+  | plus₁ _ _ IH₀ IH₁
+  | plus₂ _ _ IH₀ IH₁
+  | lets _ _ IH₀ IH₁
+  | let𝕔 _ _ IH₀ IH₁ =>
+    simp; constructor
+    apply IH₀; apply Hclosed.left
+    apply IH₁; apply Hclosed.right
+  | lit₁ => simp
+
+lemma subst_closed_id : ∀ x e v, closed_at e x → subst x v e = e :=
+  by
+  intros x e v He
+  induction e with
+  | bvar => simp
+  | fvar => simp at *; omega
+  | lam₁ _ IH
+  | lift _ IH
+  | lam𝕔 _ IH
+  | code _ IH
+  | reflect _ IH =>
+    simp; apply IH; apply He
+  | app₁ _ _ IH₀ IH₁
+  | app₂ _ _ IH₀ IH₁
+  | plus₁ _ _ IH₀ IH₁
+  | plus₂ _ _ IH₀ IH₁ =>
+    simp; constructor
+    apply IH₀; apply He.left
+    apply IH₁; apply He.right
+  | lets _ _ IHb IHe
+  | let𝕔 _ _ IHb IHe =>
+    simp; constructor
+    apply IHb; apply He.left
+    apply IHe; apply He.right
+  | lit₁ => simp
+
+lemma openSubst_intro : ∀ x e v, closed_at e x → subst x v (open₀ x e) = open_subst v e :=
+  by
+  intros _ _ _ Hclosed
+  apply subst_intro
+  apply Hclosed
+
+lemma closedb_inc: ∀ t i j,
+    closedb_at t i → i <= j →
+    closedb_at t j := by
+  intros t i j Hclose HLe
+  induction t generalizing i j with
+  | bvar => simp at *; omega
+  | fvar => simp
+  | lam₁ _ IH
+  | lift _ IH
+  | lam𝕔 _ IH
+  | code _ IH
+  | reflect _ IH =>
+    apply IH; apply Hclose; omega
+  | app₁ _ _ IH₀ IH₁
+  | app₂ _ _ IH₀ IH₁
+  | plus₁ _ _ IH₀ IH₁
+  | plus₂ _ _ IH₀ IH₁
+  | lets _ _ IH₀ IH₁
+  | let𝕔 _ _ IH₀ IH₁ =>
+    apply And.intro
+    . apply IH₀; apply Hclose.left; omega
+    . apply IH₁; apply Hclose.right; omega
+  | lit₁ => simp
+
+lemma closed_inc : ∀ x y e, closed_at e x → x <= y → closed_at e y :=
+  by
+  intros x y e Hclose Hxy
+  induction e with
+  | bvar j => simp
+  | fvar z => simp at *; omega
+  | app₁ _ _ IH₀ IH₁
+  | app₂ _ _ IH₀ IH₁
+  | plus₁ _ _ IH₀ IH₁
+  | plus₂ _ _ IH₀ IH₁
+  | lets _ _ IH₀ IH₁
+  | let𝕔 _ _ IH₀ IH₁ =>
+    simp; constructor
+    apply IH₀; apply Hclose.left
+    apply IH₁; apply Hclose.right
+  | lit₁ => simp
+  | lam₁ _ IH
+  | lift _ IH
+  | lam𝕔 _ IH
+  | code _ IH
+  | reflect _ IH =>
+    simp; apply IH; apply Hclose
+
+lemma subst_closedb_at : ∀ x e v i, closedb_at v i → closedb_at e i → closedb_at (subst x v e) i :=
+  by
+  intros x e v i Hv He
+  induction e generalizing i with
+  | bvar => apply He
+  | fvar y =>
+    by_cases HEq : x = y
+    . rw [HEq]; simp; apply Hv
+    . simp; rw [if_neg HEq]; simp
+  | lam₁ _ IH
+  | lift _ IH
+  | lam𝕔 _ IH =>
+    apply IH; apply closedb_inc; apply Hv; omega; apply He
+  | app₁ _ _ IH₀ IH₁
+  | app₂ _ _ IH₀ IH₁
+  | plus₁ _ _ IH₀ IH₁
+  | plus₂ _ _ IH₀ IH₁ =>
+    constructor
+    apply IH₀; apply Hv; apply He.left
+    apply IH₁; apply Hv; apply He.right
+  | lets _ _ IHb IHe
+  | let𝕔 _ _ IHb IHe =>
+    constructor
+    apply IHb; apply Hv; apply He.left
+    apply IHe; apply closedb_inc; apply Hv; omega; apply He.right
+  | code _ IH
+  | reflect _ IH =>
+    simp; apply IH; apply Hv; apply He
+  | lit₁ => simp
+
+lemma subst_closed_at : ∀ x e v y, closed_at v y → closed_at e y → closed_at (subst x v e) y :=
+  by
+  intros x e v y Hv He
+  induction e generalizing y with
+  | bvar => apply He
+  | fvar z =>
+    by_cases HEq : x = z
+    . rw [HEq]; simp; apply Hv
+    . simp; rw [if_neg HEq]; apply He
+  | lam₁ _ IH
+  | lift _ IH
+  | lam𝕔 _ IH =>
+    apply IH; apply Hv; apply He
+  | app₁ _ _ IH₀ IH₁
+  | app₂ _ _ IH₀ IH₁
+  | plus₁ _ _ IH₀ IH₁
+  | plus₂ _ _ IH₀ IH₁
+  | lets _ _ IH₀ IH₁
+  | let𝕔 _ _ IH₀ IH₁ =>
+    constructor
+    apply IH₀; apply Hv; apply He.left
+    apply IH₁; apply Hv; apply He.right
+  | code _ IH
+  | reflect _ IH =>
+    simp; apply IH; apply Hv; apply He
+  | lit₁ => simp
+
+lemma subst_closed_at_dec : ∀ x e v, closed_at v x → closed_at e (x + 1) → closed_at (subst x v e) x :=
+  by
+  intros x e v Hv He
+  induction e with
+  | bvar => apply He
+  | fvar z =>
+    by_cases HEq : x = z
+    . rw [← HEq]; simp; apply Hv
+    . simp; rw [if_neg HEq]; simp at *; omega
+  | lam₁ _ IH
+  | lift _ IH
+  | lam𝕔 _ IH =>
+    apply IH; apply He
+  | app₁ _ _ IH₀ IH₁
+  | app₂ _ _ IH₀ IH₁
+  | plus₁ _ _ IH₀ IH₁
+  | plus₂ _ _ IH₀ IH₁
+  | lets _ _ IH₀ IH₁
+  | let𝕔 _ _ IH₀ IH₁ =>
+    constructor
+    apply IH₀; apply He.left
+    apply IH₁; apply He.right
+  | code _ IH
+  | reflect _ IH =>
+    simp; apply IH; apply He
+  | lit₁ => simp
+
+lemma open_closedb : ∀ t n m,
+  closedb_at (opening m (.fvar n) t) m →
+  closedb_at t (m + 1) := by
+  intros t; induction t <;> intros n m h <;> simp
+  case bvar x =>
+    by_cases hx: (x = m)
+    . omega
+    . by_cases hx': (x < m)
+      . omega;
+      . simp at h; rw [if_neg hx] at h; simp at h; omega
+  case lam₁ t ih =>
+    apply ih n (m + 1); simp at h; assumption
+  case code _ ih
+     | reflect _ ih
+     | lam𝕔 _ ih
+     | lift t ih =>
+    simp at *; apply ih; apply h
+  case app₁ t1 t2 ih1 ih2
+     | app₂ t1 t2 ih1 ih2
+     | plus₁ _ _ ih1 ih2
+     | plus₂ _ _ ih1 ih2 =>
+    apply And.intro; apply ih1 n m h.1; apply ih2 n m h.2
+  case lets _ _ ih1 ih2
+     | let𝕔 _ _ ih1 ih2 =>
+    apply And.intro; apply ih1 n m h.1; apply ih2 n (m + 1) h.2
+
+lemma open_closedb': ∀ t n m,
+    closedb_at t (m + 1) → closedb_at (opening m (.fvar n) t) m := by
+  intros t; induction t <;> intros n m h <;> simp
+  case bvar x =>
+    by_cases hx: (x = m)
+    . simp [hx]
+    . rw [if_neg hx]; simp at h; simp; omega
+  case lam₁ t ih =>
+    apply ih n (m + 1); simp at h; assumption
+  case code _ ih
+     | reflect _ ih
+     | lam𝕔 _ ih
+     | lift t ih =>
+    simp at *; apply ih; apply h
+  case app₁ t1 t2 ih1 ih2
+     | app₂ t1 t2 ih1 ih2
+     | plus₁ _ _ ih1 ih2
+     | plus₂ _ _ ih1 ih2 =>
+    apply And.intro; apply ih1 n m h.1; apply ih2 n m h.2
+  case lets _ _ ih1 ih2
+     | let𝕔 _ _ ih1 ih2 =>
+    apply And.intro; apply ih1 n m h.1; apply ih2 n (m + 1) h.2
+
+theorem close_closed : ∀ e x i, closed_at e (x + 1) → closed_at (closing i x e) x :=
+  by
+  intros e x i
+  induction e generalizing i with
+  | fvar y =>
+    by_cases HEq : x = y
+    . rw [HEq]; simp
+    . simp; rw [if_neg HEq]; simp; omega
+  | bvar => simp
+  | lam₁ _ IH
+  | lift _ IH
+  | lam𝕔 _ IH
+  | code _ IH
+  | reflect _ IH =>
+    apply IH
+  | app₁ _ _ IH₀ IH₁
+  | app₂ _ _ IH₀ IH₁
+  | plus₁ _ _ IH₀ IH₁
+  | plus₂ _ _ IH₀ IH₁
+  | lets _ _ IH₀ IH₁
+  | let𝕔 _ _ IH₀ IH₁ =>
+    intro Hclose; constructor
+    apply IH₀; apply Hclose.left
+    apply IH₁; apply Hclose.right
+  | lit₁ => simp
+
+theorem open_subst_closed : ∀ x e v i, closed_at e x → closed_at v x → closed_at (opening i v e) x :=
+  by
+  intros x e v i He Hv
+  induction e generalizing i with
+  | bvar j =>
+    simp; by_cases HEq : j = i
+    . rw [if_pos HEq]; apply Hv
+    . rw [if_neg HEq]; simp
+  | fvar => apply He
+  | lit₁ => simp
+  | lam₁ _ IH
+  | lift _ IH
+  | lam𝕔 _ IH
+  | code _ IH
+  | reflect _ IH =>
+    apply IH; apply He
+  | app₁ _ _ IH₀ IH₁
+  | app₂ _ _ IH₀ IH₁
+  | plus₁ _ _ IH₀ IH₁
+  | plus₂ _ _ IH₀ IH₁
+  | lets _ _ IH₀ IH₁
+  | let𝕔 _ _ IH₀ IH₁ =>
+    constructor
+    apply IH₀; apply He.left
+    apply IH₁; apply He.right
+
+theorem open_closed : ∀ e x i, closed_at e x → closed_at (opening i (.fvar x) e) (x + 1) :=
+  by
+  intros e x i
+  induction e generalizing i with
+  | fvar y => simp; omega
+  | bvar j =>
+    by_cases HEq : j = i
+    . rw [HEq]; simp
+    . simp; rw [if_neg HEq]; simp
+  | lam₁ _ IH
+  | lift _ IH
+  | lam𝕔 _ IH
+  | code _ IH
+  | reflect _ IH =>
+    apply IH
+  | app₁ _ _ IH₀ IH₁
+  | app₂ _ _ IH₀ IH₁
+  | plus₁ _ _ IH₀ IH₁
+  | plus₂ _ _ IH₀ IH₁
+  | lets _ _ IH₀ IH₁
+  | let𝕔 _ _ IH₀ IH₁ =>
+    intro Hclose; constructor
+    apply IH₀; apply Hclose.left
+    apply IH₁; apply Hclose.right
+  | lit₁ => simp
+
+theorem close_closedb : ∀ e x i j, j < i → closedb_at e i → closedb_at (closing j x e) i :=
+  by
+  intros e x i j Hlt
+  induction e generalizing i j with
+  | fvar y =>
+    by_cases HEq : x = y
+    . rw [HEq]; simp; omega
+    . simp; rw [if_neg HEq]; simp
+  | bvar => simp
+  | lam₁ _ IH
+  | lift _ IH
+  | lam𝕔 _ IH
+  | code _ IH
+  | reflect _ IH =>
+    apply IH; omega
+  | app₁ _ _ IH₀ IH₁
+  | app₂ _ _ IH₀ IH₁
+  | plus₁ _ _ IH₀ IH₁
+  | plus₂ _ _ IH₀ IH₁
+  | lets _ _ IH₀ IH₁
+  | let𝕔 _ _ IH₀ IH₁ =>
+    intro Hclose; constructor
+    apply IH₀; omega; apply Hclose.left
+    apply IH₁; omega; apply Hclose.right
+  | lit₁ => simp
+
+lemma closedb_opening_id: ∀ t1 t2 n,
+  closedb_at t1 n → opening n t2 t1 = t1 := by
+  intros t1; induction t1 <;> intros t2 n h <;> simp
+  case bvar x => intro xn; simp at h; omega
+  case lam₁ t ih
+     | lift t ih =>
+    simp at h; apply ih; assumption
+  case code _ ih
+     | reflect _ ih
+     | lam𝕔 _ ih =>
+    simp at *; apply ih; apply h
+  case app₁ t1 t2 ih1 ih2
+     | app₂ t1 t2 ih1 ih2
+     | plus₁ _ _ ih1 ih2
+     | plus₂ _ _ ih1 ih2
+     | lets _ _ ih1 ih2
+     | let𝕔 _ _ ih1 ih2 =>
+    apply And.intro; apply ih1; apply h.1; apply ih2; apply h.2
+
+lemma open_close_id : ∀ i e x, closedb_at e i → opening i (.fvar x) (closing i x e) = e :=
+  by
+  intros i e x Hlc
+  induction e generalizing i with
+  | bvar j =>
+    simp
+    intro HEq
+    rw [HEq] at Hlc
+    simp at Hlc
+  | fvar y =>
+    simp
+    by_cases HEq : x = y
+    . rw [HEq]; simp
+    . rw [if_neg HEq]; simp
+  | lam₁ _ IHe
+  | lift _ IHe
+  | lam𝕔 _ IHe
+  | code _ IHe
+  | reflect _ IHe =>
+    simp; apply IHe; apply Hlc
+  | app₁ _ _ IH₀ IH₁
+  | app₂ _ _ IH₀ IH₁
+  | plus₁ _ _ IH₀ IH₁
+  | plus₂ _ _ IH₀ IH₁
+  | lets _ _ IH₀ IH₁
+  | let𝕔 _ _ IH₀ IH₁ =>
+    simp; constructor
+    apply IH₀; apply Hlc.left
+    apply IH₁; apply Hlc.right
+  | lit₁ => rfl
+
+lemma open_close_id₀ : ∀ e x, lc e → open₀ x (close₀ x e) = e := by apply open_close_id
+
+lemma close_open_id : ∀ i e x, closed_at e x → closing i x (opening i (.fvar x) e) = e :=
+  by
+  intros i e x Hclose
+  induction e generalizing i with
+  | bvar j =>
+    by_cases HEq : j = i
+    . simp; rw [if_pos HEq]; simp; omega
+    . simp; rw [if_neg HEq]; simp
+  | fvar y => simp at *; omega
+  | lam₁ _ IHe
+  | lift _ IHe
+  | lam𝕔 _ IHe
+  | code _ IHe
+  | reflect _ IHe =>
+    simp; apply IHe; apply Hclose
+  | app₁ _ _ IH₀ IH₁
+  | app₂ _ _ IH₀ IH₁
+  | plus₁ _ _ IH₀ IH₁
+  | plus₂ _ _ IH₀ IH₁
+  | lets _ _ IH₀ IH₁
+  | let𝕔 _ _ IH₀ IH₁ =>
+    simp; constructor
+    apply IH₀; apply Hclose.left
+    apply IH₁; apply Hclose.right
+  | lit₁ => rfl
+
+lemma close_open_id₀ : ∀ e x, closed_at e x → close₀ x (open₀ x e) = e := by apply close_open_id
+
+lemma subst_opening_comm :
+    ∀ x y e v i, x ≠ y → closedb_at v i → subst x v (opening i (.fvar y) e) = opening i (.fvar y) (subst x v e) :=
+  by
+  intro x y e v i HNe Hclosedb
+  induction e generalizing i with
+  | bvar j =>
+    by_cases HEq : j = i
+    . simp; rw [if_pos HEq]; simp; omega
+    . simp; rw [if_neg HEq]; simp
+  | fvar z =>
+    by_cases HEq : x = z
+    . simp; rw [if_pos HEq]; rw [closedb_opening_id]; apply Hclosedb
+    . simp; rw [if_neg HEq]; simp
+  | app₁ _ _ IH₀ IH₁
+  | app₂ _ _ IH₀ IH₁
+  | plus₁ _ _ IH₀ IH₁
+  | plus₂ _ _ IH₀ IH₁ =>
+    simp; constructor
+    apply IH₀; apply Hclosedb
+    apply IH₁; apply Hclosedb
+  | lets _ _ IH₀ IH₁
+  | let𝕔 _ _ IH₀ IH₁ =>
+    simp; constructor
+    apply IH₀; apply Hclosedb
+    apply IH₁; apply closedb_inc; apply Hclosedb; omega
+  | code _ IH
+  | reflect _ IH =>
+    simp; apply IH; apply Hclosedb
+  | lit₁ => simp
+  | lam₁ _ IH
+  | lift _ IH
+  | lam𝕔 _ IH =>
+    simp; apply IH; apply closedb_inc; apply Hclosedb; omega
+
+lemma subst_open₀_comm : ∀ x y e v, x ≠ y → lc v → subst x v (open₀ y e) = open₀ y (subst x v e) := by
+  intros x y e v; apply subst_opening_comm
+
+example : map𝕔₀ (.app₁ (.bvar 0) (.lam₁ (.bvar 1))) = .app₁ (.code (.bvar 0)) (.lam₁ (.code (.bvar 1))) := by simp
+
+theorem maping𝕔_intro :
+    ∀ x e i, closed_at e x → closing i x (subst x (.code (.fvar x)) (opening i (.fvar x) e)) = maping𝕔 e i :=
+  by
+  intros x e i Hclosed
+  induction e generalizing i with
+  | bvar j => by_cases HEq : j = i; rw [HEq]; simp; simp [if_neg HEq]
+  | fvar y => simp at *; by_cases HEq : x = y; omega; rw [if_neg HEq]; simp; apply HEq
+  | lam₁ _ ih
+  | lift _ ih
+  | code _ ih
+  | reflect _ ih
+  | lam𝕔 _ ih =>
+    simp at *; apply ih; apply Hclosed
+  | app₁ _ _ ih1 ih2
+  | app₂ _ _ ih1 ih2
+  | plus₁ _ _ ih1 ih2
+  | plus₂ _ _ ih1 ih2
+  | lets _ _ ih1 ih2
+  | let𝕔 _ _ ih1 ih2 =>
+    simp at *; constructor; apply ih1; apply Hclosed.left; apply ih2; apply Hclosed.right
+  | lit₁ => simp
+
+theorem map𝕔₀_intro : ∀ x e, closed_at e x → close₀ x (subst x (.code (.fvar x)) (open₀ x e)) = map𝕔₀ e :=
+  by
+  intro _ _ Hclose
+  apply maping𝕔_intro
+  apply Hclose
+
+theorem maping𝕔_closed : ∀ x e i, closed_at e x → closed_at (maping𝕔 e i) x :=
+  by
+  intros x e i He
+  induction e generalizing i with
+  | bvar j =>
+    simp; by_cases HEq : j = i
+    . rw [if_pos HEq]; apply He
+    . rw [if_neg HEq]; simp
+  | fvar => apply He
+  | lit₁ => simp
+  | lam₁ _ IH
+  | lift _ IH
+  | lam𝕔 _ IH
+  | code _ IH
+  | reflect _ IH =>
+    apply IH; apply He
+  | app₁ _ _ IH₀ IH₁
+  | app₂ _ _ IH₀ IH₁
+  | plus₁ _ _ IH₀ IH₁
+  | plus₂ _ _ IH₀ IH₁
+  | lets _ _ IH₀ IH₁
+  | let𝕔 _ _ IH₀ IH₁ =>
+    constructor
+    apply IH₀; apply He.left
+    apply IH₁; apply He.right
