CollapsingTowers/TwoLevelPCP/Env.lean
@@ -7,9 +7,79 @@ def indexr {X : Type} (n : ℕ) (l : List X) : Option X :=
   | [] => none
   | head :: tails => if tails.length == n then some head else indexr n tails
 
+theorem indexrSome : ∀ {A} (xs : List A) i,
+  i < xs.length → ∃ x, indexr i xs = some x := by
+  intro A xs i h; induction xs
+  case nil => simp at h
+  case cons x xs ih =>
+    simp; by_cases h': xs.length = i
+    . simp [h']
+    . simp [if_neg h']; apply ih; simp at h; omega
+
+theorem indexrSome' : ∀ {A} (xs : List A) i,
+  (∃ x, indexr i xs = some x) → i < xs.length := by
+  intros A xs i h; induction xs
+  case nil => simp at h
+  case cons x xs ih =>
+    simp at h; by_cases h': xs.length = i
+    . subst h'; simp
+    . simp [if_neg h'] at h; simp;
+      have h' := ih h; omega
+
 abbrev TEnv :=
   List (Ty × Stage)
 
 @[simp]
 def binds (x : ℕ) (τ : Ty) (𝕊 : Stage) (Γ : TEnv) :=
   indexr x Γ = some (τ, 𝕊)
+
+theorem binds_extend : ∀ Γ Δ x τ 𝕊, binds x τ 𝕊 Γ → binds x τ 𝕊 (Δ ++ Γ) :=
+  by
+  intros Γ Δ x τ 𝕊 Hbinds
+  induction Δ with
+  | nil => apply Hbinds
+  | cons head tails IHtails =>
+    simp
+    by_cases Hx : tails.length + Γ.length = x
+    . have Hx : x < Γ.length := by apply indexrSome'; exists (τ, 𝕊)
+      omega
+    . rw [if_neg Hx]; apply IHtails
+
+theorem binds_extendr : ∀ Γ Δ x τ 𝕊, binds x τ 𝕊 Γ → binds (x + Δ.length) τ 𝕊 (Γ ++ Δ) :=
+  by
+  intros Γ Δ x τ 𝕊
+  induction Γ with
+  | nil => simp
+  | cons head tails IHtails =>
+    simp
+    by_cases HEq : tails.length = x
+    . repeat rw [if_pos HEq]; simp
+    . repeat rw [if_neg HEq]
+      apply IHtails
+
+theorem binds_shrink : ∀ Γ Δ x τ 𝕊, x < Γ.length → binds x τ 𝕊 (Δ ++ Γ) → binds x τ 𝕊 Γ :=
+  by
+  intros Γ Δ x τ 𝕊 HLt
+  induction Δ with
+  | nil => simp
+  | cons head tails IHtails =>
+    intro Hbinds; apply IHtails
+    simp at *
+    have HNe : tails.length + Γ.length ≠ x := by omega
+    rw [if_neg HNe] at Hbinds
+    apply Hbinds
+
+theorem binds_shrinkr : ∀ Γ Δ x τ 𝕊, binds (x + Δ.length) τ 𝕊 (Γ ++ Δ) → binds x τ 𝕊 Γ :=
+  by
+  intros Γ Δ x τ 𝕊
+  induction Γ with
+  | nil =>
+    simp; intro Hindexr
+    have : x + Δ.length < Δ.length := by apply indexrSome'; exists (τ, 𝕊)
+    omega
+  | cons head tails IHtails =>
+    simp
+    by_cases HEq : tails.length = x
+    . repeat rw [if_pos HEq]; simp
+    . repeat rw [if_neg HEq]
+      apply IHtails
